\subsection{Vieta's Law}
For $a_{n}x^{n}+a_{n-1}x^{n-1}+\cdots +a_{1}x+a_{0}=0$:
\begin{itemize}
	\item $\sum x_i=-\dfrac{a_{n-1}}{a_n}$
	\item $\sum x_ix_j=\dfrac{a_{n-2}}{a_n}$
	\item $\sum x_ix_jx_k = -\dfrac{a_{n-3}}{a_n}$
	\item $\sum _{1\leq i_{1}<i_{2}<\cdots <i_{k}\leq n}\left(\prod _{j=1}^{k}r_{i_{j}}\right)=(-1)^{k}{\frac {a_{n-k}}{a_{n}}}$
	\item $\prod x_i=(-1)^n\dfrac{a_0}{a_n}$
\end{itemize}
\subsection{Summation formulae}
\subsubsection{Summation of squares}
$\sum_{r=1}^{n} r^2=\dfrac{n(n+1)(2n+1)}{6}$ 
\subsubsection{Summation of cubes}
$\sum_{r=1}^{n} r^3=\dfrac{(n(n+1))^2}{4}$
\subsection{Maclaurin series}