\section{Hyperbolic function definitions}
\subsection{$\sinh x$}
\begin{description}
	\item[Definition] $\sinh x = \dfrac{e^x-e^{-x}}{2}$
	\item[Domain] $x \in \textbf{R}$
	\item[Asymptotes] $x\rightarrow +\infty$, $y\rightarrow\dfrac{e^x}{2}$; $x\rightarrow -\infty$, $y\rightarrow -\dfrac{e^{-x}}{2}$
	\item[x-intercept] $(0,0)$
	\item[y-intercept] $(0,0)$
	\item[Graph]
\end{description}

\subsection{$\cosh x$}
\begin{description}
	\item[Definition] $\cosh x = \dfrac{e^x+e^{-x}}{2}$
	\item[Domain] $x \in \textbf{R}$
	\item[Asymptotes] $x\rightarrow +\infty$, $y\rightarrow\dfrac{e^x}{2}$; $x\rightarrow -\infty$, $y\rightarrow\dfrac{e^{-x}}{2}$
	\item[x-intercept] No
	\item[y-intercept] $(0,1)$
	\item[Graph]
\end{description}

\subsection{$\tanh x$}
\begin{description}
	\item[Definition] $\tanh x = \dfrac{\sinh x}{\cosh x}=\dfrac{e^x-e^{-x}}{e^x+e^{-x}}$
	\item[Domain] $x \in \textbf{R}$
	\item[Asymptotes] $x\rightarrow +\infty$, $y\rightarrow 1$; $x\rightarrow -\infty$, $y\rightarrow -1$
	\item[x-intercept] $(0,0)$
	\item[y-intercept] $(0,0)$
	\item[Graph]
\end{description}

\subsection{$\csch x$}
\begin{description}
	\item[Definition] $\csch x = \dfrac{1}{\sinh x}$
	\item[Domain] 
	\item[Asymptotes] 
	\item[x-intercept] 
	\item[y-intercept] 
	\item[Graph]
\end{description}


\subsection{$\sech x$}
\begin{description}
	\item[Definition] $\sech x = \dfrac{1}{\cosh x}$
	\item[Domain] 
	\item[Asymptotes] 
	\item[x-intercept] 
	\item[y-intercept] 
	\item[Graph]
\end{description}


\subsection{$\coth x$}
\begin{description}
	\item[Definition] $\coth x = \dfrac{\cosh x}{\sinh x}$
	\item[Domain] 
	\item[Asymptotes] 
	\item[x-intercept] 
	\item[y-intercept] 
	\item[Graph]
\end{description}

\section{Identities of hyperbolic functions}
Similar to trigonometric identities:
\begin{itemize}
	\item $\tanh x = \dfrac{\sinh x}{\cosh x}$
	\item $\cosh^2 x - \sinh^2 x = 1$
	\item $\tanh^2 x + \sech^2 x= 1$
	\item $\coth^2 x - \csch^2 x = 1$
\end{itemize}

\subsection{Addition}
\begin{itemize}
	\item $\sinh(x+y)=\sinh x \cosh y + \sinh y \cosh x$
	\item $\cosh(x+y)=\cosh x \cosh y + \sinh x \sinh y$
	\item $\tanh(x+y) = \dfrac{\sinh(x+y)}{\cosh(x+y)} = \dfrac{\sinh x \cosh y + \sinh y \cosh x}{\cosh x \cosh y + \sinh x \sinh y} = \dfrac{\frac{\sinh x}{\cosh x}+\frac{\sinh y}{\cosh y}}{1 + \frac{\sinh x \sinh y}{\cosh x \cosh y}}=\dfrac{\tanh x + \tanh y}{1 + \tanh x \tanh y}$
\end{itemize}

\subsection{Double angle}
\begin{itemize}
	\item $\sinh 2x = 2\sinh x \cosh x$
	\item $\cosh 2x = \cosh^2 x + \sinh^2 x = 2\cosh^2 x - 1 = 2\sinh^2 + 1$
	\item $\tanh 2x = \dfrac{2\tanh x}{1 + \tanh^2 x}$
\end{itemize}

\subsection{Power descending}


\section{Differentiating hyperbolic functions}
\begin{itemize}
	\item $(\sinh x)'=\cosh x$
	\item $(\cosh x)'=\sinh x$
	\item $(\tanh x)'=1-\tanh^2 x = \sech^2 x$
	\item $(\csch x)'=-\coth x \csch x$
	\item $(\sech x)'=-\sech x \tanh x$
	\item $(\coth x)'=-\sech^2 x$
\end{itemize}