\section{Definition}
$\int_{a}^{b} f(x) \: dx = \lim\limits_{\delta x\rightarrow0}\sum_{x=a}^{b}f(x)\delta x$

\section{Formulae}
\subsection{Integrating trigonometric functions}
\begin{itemize}
    \item $\int\sin x \dx = -\cos x + c$
    \item $\int\cos x \dx = \sin x + c$
    \item $\int \tan x \dx = -\ln |\cos x| + c= \ln |\sec x| + c$
    \item $\int \cot x \dx = \ln |\sin x| + c = -\ln |\csc x| + c$
    \item $\int \sec x \dx = \int \frac{\sec x(\sec x + \tan x)}{\sec x + \tan x} \dx = \ln |\sec x + \tan x| + c = \ln \left|\tan\left(\frac{1}{2}x+\frac{1}{4}\pi \right)\right| + c$
    \item $\int \csc x \dx = -\ln|\csc x + \cot x| + c = \ln \left|\tan\left(\frac{1}{2}x\right)\right| + c$
    \item $\int \sin^2 x \dx = \int \frac{1-\cos 2x}{2} \dx = \frac{2x-\sin 2x}{4} + c$
    \item $\int \cos^2 x \dx = \int \frac{1+\cos 2x}{2} \dx = \frac{2x+\sin 2x}{4} + c$
    \item $\int \tan^2 x \dx = \int \sec^2 x -1 \dx = \tan x - x + c$
    \item $\int \cot^2 x \dx = \int \csc^2 x -1 \dx = -\cot x - x + c$
    \item $\int \sin x \cos x \dx = \int \frac{\sin 2x}{2} \dx = -\dfrac{\cos 2x}{4} + c$
    \item $\int \tan x \sec x \dx = \sec x + c$
    \item $\int \cot x \csc x \dx = -\csc x + c$
\end{itemize}
Integrating $\sin^2x$ or $\cos^2x$ (power descending):
\begin{itemize}
    \item $\int \sin ^2 x \: dx=\int \dfrac{1-\cos 2x}{2} \: dx=\dfrac{1}{2}\left(x-\dfrac{\sin 2x}{2}\right)+c$
    \item $\int \cos ^2 x \: dx=\int \dfrac{1+\cos 2x}{2} \: dx= \dfrac{1}{2}\left(x+\dfrac{\sin 2x}{2}\right)+c$
\end{itemize}
By part:
\begin{itemize}
    \item $\int \ln x \: dx = x\ln x + x + c$
\end{itemize}
\section{Techniques}
\subsection{U-sub}
\begin{itemize}
    \item $\int f'(ax+b) \: dx = \dfrac{f(ax+b)}{a}+c$
          \begin{description}
              \item[Substitution:] $u=ax+b$
          \end{description}
    \item $\int \dfrac{f'(x)}{f(x)} \: dx = \ln |f(x)|+c$
          \begin{description}
              \item[Substitution:] $u=f(x)$
          \end{description}
\end{itemize}
\subsection{By part}
\begin{itemize}
    \item $\int u \: dv = uv - \int v \: du$
    \item LIPET rule: leftmost = $u$
        \begin{description}
            \item[L:] logarithmic
            \item[I:] inverse trigonometry
            \item[P:] polynomial
            \item[E:] exponential
            \item[T:] trigonometry
        \end{description}
\end{itemize}