$f'(x) = \lim\limits_{n \to 0}\dfrac{f(x+h)-f(x)}{h}$

\section{Formulae}
\begin{tabular}{ll}
    $\mathbf{f(x)}$ & $\mathbf{f'(x)}$      \\
    $\tan kx$       & $k\sec^2 kx$          \\
    $\sec kx$       & $k\sec kx \tan kx$    \\
    $\cot kx$       & $-k\cosec^2 kx$       \\
    $\cosec kx$     & $-k\cosec kx \cot kx$ \\
\end{tabular}

\section{Rules}
\begin{description}
    \item[Chain rule:] $\dfrac{dy}{dx} = \dfrac{dy}{du} \times \dfrac{du}{dx}$
    \item[Product rule:] $(f(x)g(x))'=f'(x)g(x)+g'(x)f(x)$
    \item[Quotient rule:] $\dfrac{f(x)}{g(x)} = \dfrac{f'(x)g(x)-g'(x)f(x)}{g^2(x)}$
\end{description}


\section{Tangent and normal}
For curve $y=f(x)$:
\begin{description}
    \item[Tangent at $(a,f(a))$:] $y-f(a)=f'(a)(x-a)$
    \item[Normal at $(a,f(a))$:] $y-f(a)=-\dfrac{1}{f'(a)}(x-a)$
\end{description}