\section{Types of differential equations}

\subsection{Order}
\begin{description}
    \item[First order] $\dv{y}{x}$
    \item[Second order] $\dv[2]{y}{x}$
    \item[$n$th order] $\dv[n]{y}{x}$
\end{description}

\subsection{Homogeneous / non-homogeneous}
\begin{description}
    \item[Homogeneous differential equations] 
    \item[Non-homogeneous differential equations] 
\end{description}

\section{First order differential equations}
\subsection{Separation}
\begin{itemize}
    \item Try to separate the equation into $f(y)\dy = g(x)\dx$
    \item Integrate both sides
\end{itemize}

\subsection{The integrating factor}
A first order differential equation of the form $\dv{y}{x}+P(x)y = Q(x)$ can be solved by multiplying every term by the integrating factor $I=e^{\int P(x)dx}$
\begin{example}
    Find the general solution of the differential equation $$\dv{y}{x}-4y=e^x$$
\end{example}
\begin{solution}
    The integrating factor is $e^{\int (-4) dx}=e^{-4x}$
    \begin{flalign*}
        e^{-4x}\dv{y}{x}-4e^{-4x}y & =e^xe^{-4x}                   \\
        \frac{\mathrm{d}}{\dx}(e^{-4x}y)         & =e^{-3x}                      \\
        e^{-4x}y                        & = \int e^{-4x} \: dx          \\
        \nonumber                       & = -\frac{1}{3}e^{-3x} + c     \\
        y                               & = -\frac{1}{3}e^{x} + ce^{4x}
    \end{flalign*}
\end{solution}

\subsection{$u$-substitution}
$$\dv{y}{x} + P(x)y = Q(x)y^n$$
\begin{enumerate}
    \item Divide by $y^n$
    \item $u$-sub: $u=y^{1-n}$
    \item Change into first order linear differential differential equation
\end{enumerate}

\section{Second order homogeneous differential equations}
$$a\dv[2]{y}{x} + b\dv{y}{x} + cy = 0$$
\begin{enumerate}
    \item Use $u$-sub: $u=\ln x$, $x=e^u$
    \item Convert into $\dv[2]{y}{u} = f(y)$
\end{enumerate}

\section{Second order non-homogeneous differential equations}

